### Formula $(x+y)^n=\sum_{k=0}^n\binom{n}{k}x^{n-k}y^{k}$
$=\sum_{k=0}^n\binom{n}{k}x^{k}y^{n-k}$ 
- $\binom{n}{k}$ is [[Binomial Coefficient]]
- [[Term]] count is $n+1$
> [!example] $(x-2)^3$, so $x=x,\ y=-2,\ n=3$
> $\large\sum_{k=0}^n\frac{3!}{(3-k)!k!}x^{3-k}y^k$
> $k=0,1,2,3$, evaluates to $x^3,-6x^2,12x,-8$
youtu.be/s19dWIHficY
### Simplifications
- $\large\binom{n}{k}=\binom{n}{n-k}$
- $\large2^n=\sum_{k=0}^n\binom{n}{k}$
- $\large\binom{n}{k}=\binom{n-1}{k}+\binom{n-1}{k-1}$ `pascal's identity`
- $\large\sum_{k=0}^n\binom{n}{k}^2=\binom{2n}{n}$
- $\large\sum_{k=0}^r\binom{m}{k}\binom{n}{r-k}=\binom{m+n}{r}$`vandermonde's identity`
